

Actividad 3

1)

$$a) e^{z^3} = e^{r^3} e^{i3\theta}$$

$$= e^{r^3} (\cos 3\theta + i \sin 3\theta)$$

$$= e^{r^3} \cos 3\theta [\cos(r^3 \sin 3\theta) + i \sin(r^3 \sin 3\theta)]$$

$$= e^{r^3} \cos^3 \theta [\cos(r^3 \sin 3\theta) + i \sin(r^3 \sin 3\theta)]$$

$$b) e^{-\frac{\pi}{4} z} : \text{ usando } z = x + iy$$

$$= \frac{e^{-\frac{\pi}{4}x - \frac{\pi}{4}y}}{4}$$

$$= \frac{e^{-\frac{\pi}{4}x - \frac{\pi}{4}y}}{4} \left[\cos\left(-\frac{\pi y}{4}\right) + i \sin\left(-\frac{\pi y}{4}\right) \right]$$

$$= \frac{e^{-\frac{\pi}{4}x}}{4} \cos\left(\frac{\pi y}{4}\right) - i \sin\left(\frac{\pi y}{4}\right)$$

Actividad 3

2)

(a) $\cos(1.7 + 1.7i)$

$$\frac{e^{i(1.7+1.7i)} + e^{-i(1.7+1.7i)}}{2}$$

$Z = re^{i\theta} \quad r = |Z| \quad Z = 1.7 + 1.7i$

$$r = \sqrt{(1.7)^2 + 1.7^2} = \sqrt{2(1.7)^2} = 1.7\sqrt{2}$$

$$\theta = \arctg\left(\frac{1.7}{1.7}\right) = \arctg(1) = \frac{\pi}{4}$$

Entonces $1.7 + 1.7i = 1.7\sqrt{2} e^{i\pi/4}$

Euler $e^{i\theta} = \cos(\theta) + i \sin(\theta)$

$$e^{i(1.7+1.7i)} = e^{i \cdot 1.7} \cdot e^{1.7i}$$

$$e^{i \cdot 1.7} = \cos(1.7) + i \sin(1.7)$$

$$e^{1.7i} = \cos(-1.7) + i \sin(-1.7) = \cos(1.7) - i \sin(1.7)$$

$$\cos(1.7 + 1.7i) = \cos(1.7) \cdot \frac{e^{-1.7} + e^{1.7}}{2} + i \sin(1.7) \cdot \frac{e^{-1.7} - e^{1.7}}{2}$$

b $\text{Sen}(2 + 13i)$

$$\text{Sen}(z) = \frac{e^{iz} - e^{-iz}}{2i}$$

$$\text{Sen}(2 + 13i) = \frac{e^{i(2+13i)} - e^{-i(2+13i)}}{2i}$$

$$e^{i(2+13i)} = e^{i \cdot 2} \cdot e^{-13}$$

$$e^{-i(2+13i)} = e^{i \cdot 2} \cdot e^{13}$$

$$e^{i \cdot 2} = \cos(2) + i \sin(2)$$

$$e^{-i \cdot 2} = \cos(-2) + i \sin(-2) = \cos(2) - i \sin(2)$$

$$\text{Sen}(2 + 13i) = (\cos(2) + i \sin(2)) \cdot e^{-13} - (\cos(2) - i \sin(2)) \cdot e^{13}$$

Actividad 3

demostrar que

3). A. $\sinh z = \sinh x \cosh y + i \cosh x \sinh y$

$$\sinh(x+iy) = \sinh x \cdot \cosh iy + \sinh iy \cdot \cosh x$$

① $\cosh(iy) = \cos y$

② $\sinh(iy) = i \sin y$

$$\sinh z = \sinh x \cosh y + i \sinh y \cdot \cosh x.$$

B. $\cos z$ es par

$$\cos z = \frac{e^{iz} + e^{-iz}}{2}$$

$$\cos(-z) = \frac{e^{i(-z)} + e^{-i(-z)}}{2}$$

$$\cos(-z) = \frac{e^{-iz} + e^{iz}}{2}$$

$$\cos(z) = \cos(-z)$$

Actividad 3

(A) A) $\cosh^2 z - \sinh^2 z = 1$

$$\cosh x = \frac{e^x + e^{-x}}{2} \quad \sinh x = \frac{e^x - e^{-x}}{2}$$

$$\left(\frac{e^z + e^{-z}}{2} \right)^2 - \left(\frac{e^z - e^{-z}}{2} \right)^2$$

$$\frac{e^{2z} + 2e^z \cdot e^{-z} + e^{-2z}}{4} - \frac{e^{2z} - 2e^z e^{-z} + e^{-2z}}{4}$$

$$\frac{e^{2z} + 2 + e^{-2z} - e^{2z} + 2 - e^{-2z}}{4}$$

$$\frac{4}{4} = 1$$

B) $\sin(z) = \sin(x) \cosh(y) + i \cos(x) \sinh(y)$

$$\sin(z) = \sin(x + iy)$$

$$\sin(x + iy) = \sin(x) \cosh(y) + i \cos(x) \sinh(y)$$

Reorganizar la expresión

$$\sin(x) \cosh(y) + i \cos(x) \sinh(y) = \sin(x) \cosh(y) + i \cos(x) \sinh(y)$$

Demostando la igualdad requerida

$$\sin(z) = \sin(x) \cosh(y) + i \cos(x) \sinh(y)$$